Sorting/MergeSortSpec.v
@@ -7,21 +7,32 @@ Set Implicit Arguments.
 
 Theorem ghms_sorted :
   forall (n : nat) (A : LinDec)
-    (s : Sort) (split : Split A)
-      (l : list A), sorted A (@ghms n A (@sort s A) split l).
+    (s : Sort A) (split : Split A)
+      (l : list A), sorted A (@ghms n A (@sort A s) split l).
 Proof.
-  intros. functional induction @ghms n A (@sort s A) split l.
+  intros. functional induction @ghms n A (@sort A s) split l.
     destruct s; cbn in *. apply sort_sorted.
     apply merge_sorted; cbn; assumption.
 Qed.
 
 Theorem ghms_perm :
   forall (n : nat) (A : LinDec)
-    (s : Sort) (split : Split A)
-      (l : list A), perm A l (@ghms n A (@sort s A) split l).
+    (s : Sort A) (split : Split A)
+      (l : list A), perm A l (@ghms n A (@sort A s) split l).
 Proof.
-  intros. functional induction @ghms n A (@sort s A) split l.
+  intros. functional induction @ghms n A (@sort A s) split l.
     destruct s; cbn in *. apply sort_perm.
     rewrite perm_split_app. rewrite e0; cbn.
       rewrite <- merge_perm; cbn. apply perm_app; assumption.
 Qed.
+Check ghms.
+
+Instance Sort_ghms
+  (n : nat) (A : LinDec) (sort : Sort A) (split : Split A) : Sort A :=
+{
+    sort := @ghms n A sort split
+}.
+Proof.
+  apply ghms_sorted.
+  apply ghms_perm.
+Defined.
