Sorting/QuicksortSpec.v
@@ -6,69 +6,8 @@ Require Import InsertionSort.
 
 Set Implicit Arguments.
 
-(*Theorem qs_perm :
-  forall (A : LinDec) (l : list A), perm A l (qs A l).
-Proof.
-  intros. functional induction qs A l.
-    auto.
-    apply perm_symm. eapply perm_trans.
-      apply perm_front.
-      apply perm_cons. unfold perm in *. intro.
-        rewrite count_app, <- IHl0, <- IHl1, <- count_filter. auto.
-Qed.
-
-Theorem qs_In :
-  forall (A : LinDec) (x : A) (l : list A),
-    In x (qs A l) <-> In x l.
-Proof.
-  intros. rewrite !count_In, <- qs_perm. reflexivity.
-Qed.
-
-Theorem qs_sorted :
-  forall (A : LinDec) (l : list A), sorted A (qs A l).
-Proof.
-  intros. functional induction qs A l.
-    constructor.
-    apply sorted_app_all.
-      assumption.
-      apply sorted_cons.
-        intros. rewrite qs_In, filter_In in H. destruct H.
-          destruct (leqb_spec x h).
-            inversion H0.
-            apply LinDec_not_leq. assumption.
-          assumption.
-      intros. rewrite qs_In, filter_In in H. destruct H.
-        destruct (leqb_spec x h); intuition.
-Qed.
-
-Instance Sort_qs : Sort :=
-{
-    sort := qs;
-    sort_sorted := qs_sorted;
-    sort_perm := qs_perm;
-}.
-
-Theorem qs2_is_qs :
-  forall (A : LinDec) (l : list A), qs2 A l = qs A l.
-Proof.
-  intros. functional induction qs2 A l.
-    compute. trivial.
-    rewrite qs_equation. rewrite bifilter_spec in e0.
-      inversion e0. rewrite H0, H1. congruence.
-Qed.
-
-Instance Sort_qs2 : Sort :=
-{
-    sort := qs2
-}.
-Proof.
-  all: intros; rewrite qs2_is_qs.
-    apply (@sort_sorted Sort_qs).
-    apply (@sort_perm Sort_qs).
-Defined.*)
-
-Theorem hqs_perm :
-  forall (n : nat) (A : LinDec) (s : Sort) (l : list A),
+(*Theorem hqs_perm :
+  forall (n : nat) (A : LinDec) (s : Sort A) (l : list A),
     perm A l (hqs n A sort l).
 Proof.
   intros. functional induction hqs n A sort l; trivial.
@@ -82,14 +21,14 @@ Proof.
 Qed.
 
 Theorem hqs_In :
-  forall (n : nat) (A : LinDec) (s : Sort) (x : A) (l : list A),
+  forall (n : nat) (A : LinDec) (s : Sort A) (x : A) (l : list A),
     In x (hqs n A sort l) <-> In x l.
 Proof.
   intros. rewrite !count_In, <- hqs_perm; auto. reflexivity.
 Qed.
 
 Theorem hqs_sorted :
-  forall (n : nat) (A : LinDec) (s : Sort) (l : list A),
+  forall (n : nat) (A : LinDec) (s : Sort A) (l : list A),
     sorted A (hqs n A sort l).
 Proof.
   intros. functional induction hqs n A sort l; trivial.
@@ -106,25 +45,25 @@ Proof.
         destruct (leqb_spec x h); intuition.
 Qed.
 
-Instance Sort_hqs (n : nat) (s : Sort) : Sort :=
+Instance Sort_hqs (n : nat) (A : LinDec) (s : Sort A) : Sort A :=
 {
-    sort := fun A : LinDec => hqs n A (@sort s A)
+    sort := hqs n A (@sort A s)
 }.
 Proof.
   intros. apply hqs_sorted.
   intros. apply hqs_perm.
-Defined.
+Defined.*)
 
-(** [ultimate_qs] specification *)
+(** [uqs] specification *)
 
-Theorem ultimate_qs_perm :
+Theorem uqs_perm :
   forall
     (A : LinDec) (small : Small A) (adhoc : AdHocSort small)
     (choosePivot : Pivot A) (partition : Partition A) (l : list A),
-      perm A l (ultimate_qs adhoc choosePivot partition l).
+      perm A l (uqs adhoc choosePivot partition l).
 Proof.
   intros.
-  functional induction @ultimate_qs A small adhoc choosePivot partition l.
+  functional induction @uqs A small adhoc choosePivot partition l.
     pose (e' := e). apply small_inl in e'; subst.
       apply adhoc_perm in e. assumption.
     assert (perm A l (pivot :: rest)).
@@ -138,25 +77,25 @@ Proof.
               rewrite partition_perm, !count_app. reflexivity.
 Qed.
 
-Theorem ultimate_qs_In :
+Theorem uqs_In :
   forall
     (A : LinDec) (small : Small A) (adhoc : AdHocSort small)
     (choosePivot : Pivot A) (partition : Partition A)
     (l : list A) (x : A),
-      In x (ultimate_qs adhoc choosePivot partition l) <->
+      In x (uqs adhoc choosePivot partition l) <->
       In x l.
 Proof.
-  intros. rewrite !count_In, <- ultimate_qs_perm; auto. reflexivity.
+  intros. rewrite !count_In, <- uqs_perm; auto. reflexivity.
 Qed.
 
-Theorem ultimate_qs_sorted :
+Theorem uqs_sorted :
   forall
     (A : LinDec) (small : Small A) (adhoc : AdHocSort small)
     (choosePivot : Pivot A) (partition : Partition A) (l : list A),
-      sorted A (ultimate_qs adhoc choosePivot partition l).
+      sorted A (uqs adhoc choosePivot partition l).
 Proof.
   intros.
-  functional induction @ultimate_qs A small adhoc choosePivot partition l.
+  functional induction @uqs A small adhoc choosePivot partition l.
     pose (e' := e). apply small_inl in e'; subst.
       apply adhoc_sorted in e. assumption.
     apply small_inr in e. apply pivot_spec in e0.
@@ -164,26 +103,53 @@ Proof.
         apply sorted_cons.
           intros. apply in_app_or in H. destruct H.
             erewrite spec_eq; eauto.
-            eapply spec_hi; eauto. eapply ultimate_qs_In; eauto.
+            eapply spec_hi; eauto. eapply uqs_In; eauto.
           apply sorted_app; auto.
             assert (forall x : A, In x eq -> x = pivot).
               eapply spec_eq; eauto.
               clear e1. induction eq; auto. destruct eq; auto. constructor.
                 rewrite (H a), (H c); cbn; auto.
                 apply IHeq. intro. inv 1; apply H; cbn; auto.
-            intros. apply ultimate_qs_In in H0.
+            intros. apply uqs_In in H0.
               erewrite (spec_eq pivot) at 1; eauto.
                 eapply spec_hi; eauto.
-          intros. apply ultimate_qs_In in H. eapply spec_lo; eauto.
+          intros. apply uqs_In in H. eapply spec_lo; eauto.
 Qed.
 
-Instance Sort_ultimate_qs
+Instance Sort_uqs
   (A : LinDec) (small : Small A) (adhoc : AdHocSort small)
-  (choosePivot : Pivot A) (partition : Partition A) : Sort' A :=
+  (choosePivot : Pivot A) (partition : Partition A) : Sort A :=
 {
-    sort' := ultimate_qs adhoc choosePivot partition
+    sort := uqs adhoc choosePivot partition
 }.
 Proof.
-  intros. apply ultimate_qs_sorted.
-  intros. apply ultimate_qs_perm.
+  intros. apply uqs_sorted.
+  intros. apply uqs_perm.
+Defined.
+
+Instance Sort_qs (A : LinDec) : Sort A :=
+{
+    sort := qs A
+}.
+Proof.
+  intros. apply uqs_sorted.
+  intros. apply uqs_perm.
+Defined.
+
+Instance Sort_qs2 (A : LinDec) : Sort A :=
+{
+    sort := qs2 A
+}.
+Proof.
+  intros. apply uqs_sorted.
+  intros. apply uqs_perm.
+Defined.
+
+Instance Sort_hqs (A : LinDec) (n : nat) (s : Sort A) : Sort A :=
+{
+    sort := hqs n s
+}.
+Proof.
+  apply uqs_sorted.
+  apply uqs_perm.
 Defined.
